src/lean/Nemonuri/Study/StanfordOnline/Compilers/Lemma/Basic.lean
@@ -10,21 +10,32 @@ set_option autoImplicit false
 variable {State Label : Type*}
 
 
-theorem Cslib.LTS.MTr.single_iff
+namespace Cslib.LTS
+
+theorem MTr.single_iff
   (lts : LTS State Label) (s1 : State) (μ : Label) (s2 : State)
   : lts.MTr s1 [μ] s2 ↔ lts.Tr s1 μ s2 :=
   Iff.intro (Cslib.LTS.MTr.single_invert lts s1 μ s2) (Cslib.LTS.MTr.single lts)
 
 
-theorem Cslib.LTS.MTr.split_iff
+theorem MTr.split_iff
   (lts : LTS State Label) {s0 : State} {μs1 μs2 : List Label} {s2 : State}
   : (lts.MTr s0 (μs1 ++ μs2) s2) ↔ (∃ s1, lts.MTr s0 μs1 s1 ∧ lts.MTr s1 μs2 s2) := by
-  open Cslib LTS Classical in
+  open Classical in
   constructor
   · intro h ; exact MTr.split h
   · intro h
     obtain ⟨_, ⟨mtrL, mtrR⟩⟩ := h
     exact Cslib.LTS.MTr.comp lts mtrL mtrR
 
+
+def IsImageNonempty (lts : LTS State Label) (s1: State) (μ : Label) : Prop :=
+  (lts.image s1 μ).Nonempty
+
+theorem isImageNonempty_iff {lts : LTS State Label} {s1: State} {μ : Label}
+  : lts.IsImageNonempty s1 μ ↔ ∃s2, lts.Tr s1 μ s2 := by
+  simp [IsImageNonempty, Set.Nonempty, Membership.mem, Set.Mem, Cslib.LTS.image, setOf]
+
+end Cslib.LTS
 
 end public_s
